

**Biostat 602 Winter 2017**

**Lecture Set 7**

**Point Estimation**

**Maximum Likelihood Estimation**

**Reading: CB 7.2**

## Maximum Likelihood Estimation

### Recap

$X_1, \dots, X_n$  *i.i.d.*  $f_X(x|\theta)$ . The joint distribution of  $\mathbf{X} = (X_1, \dots, X_n)$  is

$$f_{\mathbf{X}}(\mathbf{x}|\theta) = \prod_{i=1}^n f_X(x_i|\theta)$$

Given that  $\mathbf{X} = \mathbf{x}$  is observed, the function of  $\theta$  defined by  $L(\theta|\mathbf{x}) = f_{\mathbf{X}}(\mathbf{x}|\theta)$  is called the **likelihood function**.

For a given sample point  $\mathbf{x} = (x_1, \dots, x_n)$ , let  $\hat{\theta}(\mathbf{x})$  be the value such that  $L(\theta|\mathbf{x})$  attains its maximum. More formally,

$$L(\hat{\theta}(\mathbf{x})|\mathbf{x}) \geq L(\theta|\mathbf{x}) \quad , \forall \theta \in \Omega, \quad \text{where } \hat{\theta}(\mathbf{x}) \in \Omega.$$

$\hat{\theta}(\mathbf{x})$  is called the *maximum likelihood estimate* of  $\theta$  based on data  $\mathbf{x}$ , and

$\hat{\theta}(\mathbf{X})$  is the *maximum likelihood estimator (MLE)* of  $\theta$ .

## Strategies for finding MLE of $\theta$

There are two situations.

### If the function is differentiable with respect to $\theta$

1. Find candidates that makes first order derivative to be zero
2. Check second-order derivative to check local maximum.
  - For one-dimensional parameter,  $\frac{\partial^2 L(\theta)}{\partial \theta^2} < 0$  implies local maximum.
  - For two-dimensional parameter, we need to show
    - (a)  $\partial^2 L(\theta_1, \theta_2) / \partial \theta_1^2 < 0$  or  $\partial^2 L(\theta_1, \theta_2) / \partial \theta_2^2 < 0$ .
    - (b) Determinant of second-order derivative is positive
3. Check whether boundary gives global maximum.
  - Or clearly justify that boundaries cannot be global maximum.

### If the function is NOT differentiable with respect to $\theta$

- Use numerical methods, or
- Directly maximize using inequalities or properties of the function.

In general, one is content with MLEs that are local maximum.

### Example 1 – Normal MLEs, both parameters unknown

Let  $X_1, \dots, X_n$  be *i.i.d* observations from  $\mathcal{N}(\mu, \sigma^2)$ . Find MLE of  $(\mu, \sigma^2)$ .

Two possible approaches

- Use second-order partial derivatives and their Hessian to show global maximum
- Find a workaround to avoid complex calculations.

**Common step : Calculate first-order derivatives**

**Likelihood Function**

$$\begin{aligned}L(\mu, \sigma^2 | \mathbf{x}) &= \frac{1}{(2\pi\sigma^2)^{n/2}} \exp \left[ -\frac{1}{2} \sum_{i=1}^n \frac{(x_i - \mu)^2}{\sigma^2} \right] \\l(\mu, \sigma^2 | \mathbf{x}) &= -\frac{n}{2} \log 2\pi - \frac{n}{2} \log \sigma^2 - \frac{1}{2} \sum_{i=1}^n \frac{(x_i - \mu)^2}{\sigma^2}\end{aligned}$$

**Partial derivative with respect to  $\mu$**

$$\begin{aligned}L(\mu, \sigma^2 | \mathbf{x}) &= \frac{1}{(2\pi\sigma^2)^{n/2}} \exp \left[ -\frac{1}{2} \sum_{i=1}^n \frac{(x_i - \mu)^2}{\sigma^2} \right] \\l(\mu, \sigma^2 | \mathbf{x}) &= -\frac{n}{2} \log 2\pi - \frac{n}{2} \log \sigma^2 - \frac{1}{2} \sum_{i=1}^n \frac{(x_i - \mu)^2}{\sigma^2} \\ \frac{\partial l}{\partial \mu} &= \frac{1}{\sigma^2} \sum_{i=1}^n (x_i - \mu) = 0 \\ \hat{\mu} &= \frac{1}{n} \sum_{i=1}^n x_i = \bar{x}\end{aligned}$$

partial derivative with respect to  $\sigma^2$

$$\frac{\partial l}{\partial \sigma^2} = -\frac{n}{2\sigma^2} + \frac{1}{2\sigma^4} \sum_{i=1}^n (x_i - \mu)^2 = 0$$

$$\hat{\sigma}^2 = \frac{1}{n} \sum_{i=1}^n (x_i - \bar{x})^2$$

Checking second-order partial derivatives

With respect to  $\mu$

$$\frac{\partial^2 l}{\partial \mu^2} = -\frac{n}{\sigma^2} < 0$$

With respect to  $\sigma^2$

$$\frac{\partial^2 l}{\partial (\sigma^2)^2} = \frac{n}{2\sigma^4} - \frac{1}{\sigma^6} \sum_{i=1}^n (x_i - \mu)^2$$

With respect to both parameters

$$\frac{\partial^2 l}{\partial \mu \partial \sigma^2} = -\frac{1}{\sigma^4} \sum_{i=1}^n (x_i - \mu)$$

Calculate Hessian

$$\begin{aligned} & \left| \begin{array}{cc} \frac{\partial^2 l}{\partial \mu^2} & \frac{\partial^2 l}{\partial \mu \partial \sigma^2} \\ \frac{\partial^2 l}{\partial \mu \partial \sigma^2} & \frac{\partial^2 l}{\partial (\sigma^2)^2} \end{array} \right|_{\mu=\hat{\mu}, \sigma^2=\hat{\sigma}^2} \\ = & \left| \begin{array}{cc} -\frac{n}{\sigma^2} & -\frac{1}{\sigma^4} \sum_{i=1}^n (x_i - \mu) \\ -\frac{1}{\sigma^4} \sum_{i=1}^n (x_i - \mu) & \frac{n}{2\sigma^4} - \frac{1}{\sigma^6} \sum_{i=1}^n (x_i - \mu)^2 \end{array} \right|_{\mu=\bar{x}, \sigma^2=\hat{\sigma}^2} \\ = & \frac{1}{\sigma^6} \left[ -\frac{n^2}{2} + \frac{n}{\sigma^2} \sum_{i=1}^n (x_i - \mu)^2 - \frac{1}{\sigma^2} \left( \sum_{i=1}^n (x_i - \mu) \right)^2 \right]_{\mu=\bar{x}, \sigma^2=\hat{\sigma}^2} \\ = & \frac{1}{\hat{\sigma}^6} \left[ -\frac{n^2}{2} + \frac{n}{\hat{\sigma}^2} (n\hat{\sigma}^2) - \frac{1}{\hat{\sigma}^2} \left( \sum_{i=1}^n (x_i - \bar{x}) \right)^2 \right] = \frac{1}{\hat{\sigma}^6} \frac{n^2}{2} > 0 \end{aligned}$$

Thus, the conditions for local (interior) maximum is indeed found. Because this is a unique interior maximum, it is also a global maximum. Therefore,  $(\hat{\mu}, \hat{\sigma}^2) = (\bar{x}, \frac{1}{n} \sum_{i=1}^n (x_i - \bar{x})^2)$  is an MLE.

### A simpler workaround

First, fix one parameter, say  $\sigma^2$ .

$$l(\mu, \sigma^2 | \mathbf{x}) = -\frac{n}{2} \log 2\pi - \frac{n}{2} \log \sigma^2 - \frac{1}{2} \sum_{i=1}^n \frac{(x_i - \mu)^2}{\sigma^2}$$

If

$$\mu \neq \bar{x}, \quad \text{then} \quad \sum_{i=1}^n (x_i - \mu)^2 > \sum_{i=1}^n (x_i - \bar{x})^2$$

so  $\hat{\mu} = \bar{x}$  must hold to maximize the log-likelihood.

Second, reduce the problem into one-parameter maximization

Given  $\hat{\mu} = \bar{x}$ , the log-likelihood is maximized at  $\hat{\sigma}^2 = \frac{1}{n} \sum_{i=1}^n (x_i - \bar{x})^2$ , because

$$\frac{\partial l}{\partial \sigma^2} = -\frac{n}{2\sigma^4}(\sigma^2 - \hat{\sigma}^2)$$

is always positive when  $\sigma^2 < \hat{\sigma}^2$  and always negative when  $\sigma^2 > \hat{\sigma}^2$ . Hence  $l$  as a function of  $\sigma^2$  increases upto  $\hat{\sigma}^2$  and then decreases.

Therefore,  $(\hat{\mu}, \hat{\sigma}^2) = (\bar{x}, \frac{1}{n} \sum_{i=1}^n (x_i - \bar{x})^2)$  is an MLE.

### Example 2 – Ranged Normal with Known Variance

Let  $X_1, \dots, X_n$  i.i.d.  $\mathcal{N}(\mu, 1)$  where  $\underline{\mu \geq 0}$ . Find MLE of  $\mu$ .

**Solution:**

$$L(\mu|\mathbf{x}) = \prod_{i=1}^n \frac{1}{\sqrt{2\pi}} \exp \left[ -\frac{(x_i - \mu)^2}{2} \right] = (2\pi)^{-n/2} \exp \left[ -\frac{\sum_{i=1}^n (x_i - \mu)^2}{2} \right]$$

$$l(\mu|\mathbf{x}) = \log L(\mu, \mathbf{x}) = C - \frac{\sum_{i=1}^n (x_i - \mu)^2}{2}$$

$$\frac{\partial l}{\partial \mu} = \frac{2 \sum_{i=1}^n (x_i - \mu)}{2} = 0, \quad \frac{\partial^2 l}{\partial \mu^2} < 0$$

$$\hat{\mu} = \sum_{i=1}^n x_i / n = \bar{x}$$

**Question: ARE WE DONE?**

**The MLE parameter must be within the parameter space.**

We need to check whether  $\hat{\mu}$  is within the parameter space  $[0, \infty)$ .

- If  $\bar{x} \geq 0$ ,  $\hat{\mu} = \bar{x}$  falls into the parameter space.
- If  $\bar{x} < 0$ ,  $\hat{\mu} = \bar{x}$  does NOT fall into the parameter space.

When  $\bar{x} < 0$

$$\frac{\partial l}{\partial \mu} = \sum_{i=1}^n (x_i - \mu) = n(\bar{x} - \mu) < 0$$

for  $\mu \geq 0$ . Therefore,  $l(\mu|\mathbf{x})$  is a decreasing function of  $\mu$ . So  $\hat{\mu} = 0$  when  $\bar{x} < 0$ .

Therefore, MLE is

$$\hat{\mu}(\mathbf{X}) = \max(\bar{X}, 0)$$

### Example 3 – Binomial MLE, unknown number of trials

Let  $X_1, \dots, X_n$  be random sample from  $Binomial(k, p)$  population, where  $p$  is known and  $k$  is unknown. Find the MLE of  $k$ .

#### Likelihood Function

$$L(k|\mathbf{x}, p) = \begin{cases} \prod_{i=1}^n \binom{k}{x_i} p^{x_i} (1-p)^{k-x_i} & (k \geq \max_i x_i) \\ 0 & (k < \max_i x_i) \end{cases}$$

The likelihood function is not differentiable with respect to  $k$  because  $k$  is an integer.

So how can we find MLE?

**Idea: Instead of differentiating, take a ratio**

We want to find  $k$  such that

$$\frac{L(k|\mathbf{x}, p)}{L(k-1|\mathbf{x}, p)} \geq 1 \quad \text{and} \quad \frac{L(k+1|\mathbf{x}, p)}{L(k|\mathbf{x}, p)} < 1$$

$$\begin{aligned} \frac{L(k, \mathbf{x}, p)}{L(k-1, \mathbf{x}, p)} &= \frac{\prod_{i=1}^n \binom{k}{x_i} p^{x_i} (1-p)^{k-x_i}}{\prod_{i=1}^n \binom{k-1}{x_i} p^{x_i} (1-p)^{k-1-x_i}} \\ &= \frac{\prod_{i=1}^n \frac{k!}{x_i!(k-x_i)!} p^{x_i} (1-p)^{k-x_i}}{\prod_{i=1}^n \frac{(k-1)!}{x_i!(k-1-x_i)!} p^{x_i} (1-p)^{k-1-x_i}} \\ &= \prod_{i=1}^n \frac{k(1-p)}{k-x_i} = \frac{k^n (1-p)^n}{\prod_{i=1}^n (k-x_i)} \end{aligned}$$



## Finding MLE

Find maximum  $k$  such that  $\frac{L(k|\mathbf{x},p)}{L(k-1|\mathbf{x},p)} \geq 1$

$$\begin{aligned} k^n(1-p)^n &\geq \prod_{i=1}^n (k - x_i) \\ (1-p)^n &\geq \prod_{i=1}^n \left(1 - \frac{x_i}{k}\right) \quad (k \geq \max_i x_i) \end{aligned} \tag{1}$$

- The right-hand side is an increasing function of  $k$
- The right-hand side is  $0 < (1-p)^n$ , when  $k = \max_i x_i$ .
- The right-hand side will converge to  $1 > (1-p)^n$  as  $k \rightarrow \infty$ .
- Thus, there is a unique maximum for the likelihood function.
- $\hat{k}_{MLE}$  can be numerically solved as the maximum  $k$  satisfying (1).

**Example 4** Let  $X_1, \dots, X_n$  be a random sample from a pdf

$$f_X(x|\theta) = \theta x^{\theta-1}, \quad 0 < x < 1, \quad 0 < \theta < \infty.$$

- (a) Find method of moments estimator for  $\theta$ .
- (b) Find the MLE of  $\theta$ .

### Example 5 – Two-parameter Exponential

Let  $X_1, \dots, X_n$  be *i.i.d.* observations from a location-scale family of an exponential distribution with pdf

$$f_X(x|\theta) = \frac{1}{\sigma} \exp\left(-\frac{x - \mu}{\sigma}\right), \quad x \geq \mu, \sigma > 0$$

- (a) Find MLEs of  $\mu$  and  $\sigma$ .
- (b) Find MLE of  $S(t) = \Pr(X > t)$  for a fixed  $t$ .

## Invariance

MLE is invariant under monotonic transformation.

**Question:** If  $\hat{\theta}$  is the MLE of  $\theta$ , what is the MLE of  $\tau(\theta)$ ?

**Example 6:** Let  $X_1, \dots, X_n$  be a random sample from  $Bernoulli(p)$  where  $0 < p < 1$ .

1. What is the MLE of  $p$ ?
2. What is the MLE of odds, defined by  $\eta = p/(1 - p)$ ?

**MLE of  $p$**

$$L(p|\mathbf{x}) = \prod_{i=1}^n p^{x_i} (1 - p)^{1-x_i} = p^{\sum x_i} (1 - p)^{n - \sum x_i}$$

$$l(p|\mathbf{x}) = \log p \sum_{i=1}^n x_i + \log(1 - p) (n - \sum_{i=1}^n x_i)$$

$$\frac{\partial l}{\partial p} = \frac{\sum_{i=1}^n x_i}{p} - \frac{n - \sum_{i=1}^n x_i}{1 - p} = 0$$

$$\hat{p} = \frac{\sum_{i=1}^n x_i}{n} = \bar{x}$$

**MLE of  $\eta = \frac{p}{1-p}$**

- $\eta = p/(1 - p) = \tau(p)$
- $p = \eta/(1 + \eta) = \tau^{-1}(\eta)$

$$\begin{aligned} L^*(\eta|\mathbf{x}) &= p^{\sum x_i} (1 - p)^{n - \sum x_i} \\ &= \frac{p}{1 - p}^{\sum x_i} (1 - p)^n = \frac{\eta^{\sum x_i}}{(1 + \eta)^n} \\ l^*(\eta|\mathbf{x}) &= \sum_{i=1}^n x_i \log \eta - n \log(1 + \eta) \\ \frac{\partial l^*}{\partial \eta} &= \frac{\sum_{i=1}^n x_i}{\eta} - \frac{n}{1 + \eta} = 0 \\ \hat{\eta} &= \frac{\sum_{i=1}^n x_i/n}{1 - \sum_{i=1}^n x_i/n} = \frac{\bar{x}}{1 - \bar{x}} = \tau(\hat{p}) \end{aligned}$$

Another way to get MLE of  $\eta = \frac{p}{1-p}$

$$L^*(\eta|\mathbf{x}) = \frac{\eta^{\sum x_i}}{(1 + \eta)^n}$$

- From MLE of  $\hat{p}$ , we know  $L^*(\eta|\mathbf{x})$  is maximized when  $p = \eta/(1 + \eta) = \hat{p}$ .
- Equivalently,  $L^*(\eta|\mathbf{x})$  is maximized when  $\eta = \hat{p}/(1 - \hat{p}) = \tau(\hat{p})$ , because  $\tau$  is a one-to-one function.
- Therefore  $\hat{\eta} = \tau(\hat{p})$ .

**Result:** Denote the MLE of  $\theta$  by  $\hat{\theta}$ . If  $\tau(\theta)$  is an one-to-one function of  $\theta$ , then MLE of  $\tau(\theta)$  is  $\tau(\hat{\theta})$ .

**Proof:** The likelihood function in terms of  $\tau(\theta) = \eta$  is

$$\begin{aligned} L^*(\tau(\theta)|\mathbf{x}) &= \prod_{i=1}^n f_X(x_i|\theta) = \prod_{i=1}^n f(x_i|\tau^{-1}(\eta)) \\ &= L(\tau^{-1}(\eta)|\mathbf{x}) \end{aligned}$$

We know this function is maximized when  $\tau^{-1}(\eta) = \hat{\theta}$ , or equivalently, when  $\eta = \tau(\hat{\theta})$ . Therefore, MLE of  $\eta = \tau(\theta)$  is  $\hat{\eta} = \tau(\hat{\theta})$ .

### Induced Likelihood Function

- Let  $L(\theta|\mathbf{x})$  be the likelihood function for a given data  $x_1, \dots, x_n$ ,
- and let  $\eta = \tau(\theta)$  be a (possibly not a one-to-one) function of  $\theta$ .

We define the *induced likelihood function*  $L^*$  by

$$L^*(\eta|\mathbf{x}) = \sup_{\theta \in \tau^{-1}(\eta)} L(\theta|\mathbf{x})$$

where  $\tau^{-1}(\eta) = \{\theta : \tau(\theta) = \eta, \theta \in \Omega\}$ .

- The value of  $\eta$  that maximize  $L^*(\eta|\mathbf{x})$  is called the MLE of  $\eta = \tau(\theta)$ .

**Theorem 7.2.10:** If  $\theta$  is the MLE of  $\hat{\theta}$ , then the MLE of  $\eta = \tau(\theta)$  is  $\tau(\hat{\theta})$ , where  $\tau(\theta)$  is any function of  $\theta$ .

**Proof - Using Induced Likelihood Function**

$$\begin{aligned}
 L^*(\hat{\eta}|\mathbf{x}) &= \sup_{\eta} L^*(\eta|\mathbf{x}) = \sup_{\eta} \sup_{\theta \in \tau^{-1}(\eta)} L(\theta|\mathbf{x}) \\
 &= \sup_{\theta} L(\theta|\mathbf{x}) = L(\hat{\theta}|\mathbf{x}) \\
 L(\hat{\theta}|\mathbf{x}) &= \sup_{\theta \in \tau^{-1}(\tau(\hat{\theta}))} L(\theta|\mathbf{x}) = L^*[\tau(\hat{\theta})|\mathbf{x}]
 \end{aligned}$$

Hence,  $L^*(\hat{\eta}|\mathbf{x}) = L^*[\tau(\hat{\theta})|\mathbf{x}]$  and  $\tau(\hat{\theta})$  is the MLE of  $\tau(\theta)$ .

### Properties of MLE

1. Optimal in some sense : We will study this later
2. By definition, MLE will always fall into the range of the parameter space.
3. Not always easy to obtain; may be hard to find the global maximum.
4. Heavily depends on the underlying distributional assumptions (i.e. not robust).